[Remora] Improve handling of indices.
Distinguish dimensions and shapes syntactically, obviating the need for explicit
sorting rules.

books/kestrel/remora/abstract-syntax-derived-fixtypes.lisp
@@ -13,6 +13,7 @@
 (include-book "abstract-syntax-trees")
 
 (include-book "kestrel/fty/defresult" :dir :system)
+(include-book "kestrel/fty/string-string-map" :dir :system)
 
 (acl2::controlled-configuration)
 
@@ -38,20 +39,6 @@
 
 ;;;;;;;;;;;;;;;;;;;;;;;;;;;;;;;;;;;;;;;;;;;;;;;;;;;;;;;;;;;;;;;;;;;;;;;;;;;;;;;;
 
-(fty::defresult sort-result
-  :short "Fixtype of sorts and errors."
-  :ok sort
-  :pred sort-resultp)
-
-;;;;;;;;;;;;;;;;;;;;;;;;;;;;;;;;;;;;;;;;
-
-(fty::defresult sort-list-result
-  :short "Fixtype of (i) lists of sorts and (ii) errors."
-  :ok sort-list
-  :pred sort-list-resultp)
-
-;;;;;;;;;;;;;;;;;;;;;;;;;;;;;;;;;;;;;;;;
-
 (fty::defresult kind-result
   :short "Fixtype of kinds and errors."
   :ok kind
@@ -66,10 +53,25 @@
 
 ;;;;;;;;;;;;;;;;;;;;;;;;;;;;;;;;;;;;;;;;
 
+(fty::defresult shape-result
+  :short "Fixtype of shapes and error."
+  :ok shape
+  :pred shape-resultp)
+
+;;;;;;;;;;;;;;;;;;;;;;;;;;;;;;;;;;;;;;;;
+
+(fty::defresult shape-list-result
+  :short "Fixtype of (i) lists of shapes and (ii) error."
+  :ok shape-list
+  :pred shape-list-resultp)
+
+;;;;;;;;;;;;;;;;;;;;;;;;;;;;;;;;;;;;;;;;
+
 (fty::defresult index-result
   :short "Fixtype of indices and errors."
   :ok index
-  :pred index-resultp)
+  :pred index-resultp
+  :prepwork ((local (in-theory (enable index-kind)))))
 
 ;;;;;;;;;;;;;;;;;;;;;;;;;;;;;;;;;;;;;;;;
 
@@ -93,6 +95,116 @@
   :pred type-list-resultp)
 
 ;;;;;;;;;;;;;;;;;;;;;;;;;;;;;;;;;;;;;;;;;;;;;;;;;;;;;;;;;;;;;;;;;;;;;;;;;;;;;;;;
+
+(fty::defomap string-kind-map
+  :short "Fixtype of maps from strings to kinds."
+  :key-type string
+  :val-type kind
+  :pred string-kind-mapp)
+
+;;;;;;;;;;;;;;;;;;;;;;;;;;;;;;;;;;;;;;;;
+
+(fty::defomap string-dim-map
+  :short "Fixtype of maps from strings to dimensions."
+  :key-type string
+  :val-type dim
+  :pred string-dim-mapp)
+
+;;;;;;;;;;;;;;;;;;;;;;;;;;;;;;;;;;;;;;;;
+
+(fty::defomap string-shape-map
+  :short "Fixtype of maps from strings to shapes."
+  :key-type string
+  :val-type shape
+  :pred string-shape-mapp)
+
+;;;;;;;;;;;;;;;;;;;;;;;;;;;;;;;;;;;;;;;;
+
+(fty::defomap string-index-map
+  :short "Fixtype of maps from strings to indices."
+  :key-type string
+  :val-type index
+  :pred string-index-mapp
+
+  ///
+
+  (defrule string-index-mapp-of-from-lists
+    (implies (and (string-listp strings)
+                  (index-listp indices)
+                  (equal (len indices) (len strings)))
+             (string-index-mapp (omap::from-lists strings indices)))
+    :induct t
+    :enable (omap::from-lists string-listp)))
+
+;;;;;;;;;;;;;;;;;;;;;;;;;;;;;;;;;;;;;;;;
+
+(fty::defomap string-type-map
+  :short "Fixtype of maps from strings to types."
+  :key-type string
+  :val-type type
+  :pred string-type-mapp
+
+  ///
+
+  (defrule string-type-mapp-of-from-lists
+    (implies (and (string-listp strings)
+                  (type-listp types)
+                  (equal (len types) (len strings)))
+             (string-type-mapp (omap::from-lists strings types)))
+    :induct t
+    :enable (omap::from-lists string-listp)))
+
+;;;;;;;;;;;;;;;;;;;;;;;;;;;;;;;;;;;;;;;;;;;;;;;;;;;;;;;;;;;;;;;;;;;;;;;;;;;;;;;;
+
+(fty::defprod stringstringmap-pair
+  :short "Fixtype of pairs consisting of two maps from strings to strings."
+  ((1st string-string-map)
+   (2nd string-string-map))
+  :pred stringstringmap-pairp)
+
+;;;;;;;;;;;;;;;;;;;;
+
+(fty::defresult stringstringmap-pair-result
+  :short "Fixtype of (i) pairs consisting of two maps from strings to strings
+          and (ii) errors."
+  :ok stringstringmap-pair
+  :pred stringstringmap-pair-resultp
+  :prepwork ((local (in-theory (enable strip-cars)))))
+
+;;;;;;;;;;;;;;;;;;;;;;;;;;;;;;;;;;;;;;;;
+
+(fty::defprod type+shape
+  :short "Fixtype of pairs consisting of a type and a shape."
+  ((type type)
+   (shape shape))
+  :pred type+shape-p)
+
+;;;;;;;;;;;;;;;;;;;;
+
+(fty::defresult type+shape-result
+  :short "Fixtype of (i) pairs consisting of a type and a shape
+          and (ii) errors."
+  :ok type+shape
+  :pred type+shape-resultp)
+
+;;;;;;;;;;;;;;;;;;;;;;;;;;;;;;;;;;;;;;;;
+
+(fty::deflist type+shape-list
+  :short "Fixtype lists of pairs consisting of a type and a shape."
+  :elt-type type+shape
+  :true-listp t
+  :elementp-of-nil nil
+  :pred type+shape-listp)
+
+;;;;;;;;;;;;;;;;;;;;
+
+(fty::defresult type+shape-list-result
+  :short "Fixtype of (i) lists of pairs consisting of a type and a shape
+          and (ii) errors."
+  :ok type+shape-list
+  :pred type+shape-list-resultp)
+
+;;;;;;;;;;;;;;;;;;;;;;;;;;;;;;;;;;;;;;;;
 
 (fty::defprod type+index
   :short "Fixtype of pairs consisting of a type and an index."
@@ -144,20 +256,20 @@
 
 ;;;;;;;;;;;;;;;;;;;;;;;;;;;;;;;;;;;;;;;;
 
-(fty::defprod sortedvarlist+type
-  :short "Fixtype of pairs consisting of a list of sorted variables and a type."
-  ((vars sorted-var-list)
+(fty::defprod indexparamlist+type
+  :short "Fixtype of pairs consisting of a list of index parameters and a type."
+  ((params index-param-list)
    (type type))
-  :pred sortedvarlist+type-p)
+  :pred indexparamlist+type-p)
 
 ;;;;;;;;;;;;;;;;;;;;
 
-(fty::defresult sortedvarlist+type-result
+(fty::defresult indexparamlist+type-result
   :short "Fixtype of
-          (i) pairs consisting of a list of sorted variables and a type
+          (i) pairs consisting of a list of index parameters and a type
           and (ii) errors."
-  :ok sortedvarlist+type
-  :pred sortedvarlist+type-resultp
+  :ok indexparamlist+type
+  :pred indexparamlist+type-resultp
   :prepwork ((local (in-theory (enable strip-cars)))))
 
 ;;;;;;;;;;;;;;;;;;;;;;;;;;;;;;;;;;;;;;;;
@@ -178,64 +290,24 @@
   :pred kindedvarlist+type-resultp
   :prepwork ((local (in-theory (enable strip-cars)))))
 
-;;;;;;;;;;;;;;;;;;;;;;;;;;;;;;;;;;;;;;;;;;;;;;;;;;;;;;;;;;;;;;;;;;;;;;;;;;;;;;;;
-
-(fty::defomap string-sort-map
-  :short "Fixtype of maps from strings to sorts."
-  :key-type string
-  :val-type sort
-  :pred string-sort-mapp
-
-  ///
-
-  (defrule string-sort-mapp-of-from-lists
-    (implies (and (string-listp strings)
-                  (sort-listp sorts)
-                  (equal (len sorts) (len strings)))
-             (string-sort-mapp (omap::from-lists strings sorts)))
-    :induct t
-    :enable (omap::from-lists string-listp)))
-
 ;;;;;;;;;;;;;;;;;;;;;;;;;;;;;;;;;;;;;;;;
 
-(fty::defomap string-kind-map
-  :short "Fixtype of maps from strings to kinds."
-  :key-type string
-  :val-type kind
-  :pred string-kind-mapp)
+(fty::defprod stringdimmap+stringshapemap
+  :short "Fixtype of pairs consisting of
+          a map from strings to dimensions
+          and a map from strings to shapes."
+  ((dim-map string-dim-map)
+   (shape-map string-shape-map))
+  :pred stringdimmap+stringshapemap-p)
 
-;;;;;;;;;;;;;;;;;;;;;;;;;;;;;;;;;;;;;;;;
+;;;;;;;;;;;;;;;;;;;;
 
-(fty::defomap string-index-map
-  :short "Fixtype of maps from strings to indices."
-  :key-type string
-  :val-type index
-  :pred string-index-mapp
-
-  ///
-
-  (defrule string-index-mapp-of-from-lists
-    (implies (and (string-listp strings)
-                  (index-listp indices)
-                  (equal (len indices) (len strings)))
-             (string-index-mapp (omap::from-lists strings indices)))
-    :induct t
-    :enable (omap::from-lists string-listp)))
-
-;;;;;;;;;;;;;;;;;;;;;;;;;;;;;;;;;;;;;;;;
-
-(fty::defomap string-type-map
-  :short "Fixtype of maps from strings to types."
-  :key-type string
-  :val-type type
-  :pred string-type-mapp
-
-  ///
-
-  (defrule string-type-mapp-of-from-lists
-    (implies (and (string-listp strings)
-                  (type-listp types)
-                  (equal (len types) (len strings)))
-             (string-type-mapp (omap::from-lists strings types)))
-    :induct t
-    :enable (omap::from-lists string-listp)))
+(fty::defresult stringdimmap+stringshapemap-result
+  :short "Fixtype of
+          (i) pairs consisting of
+          a map from strings to dimensions
+          and a map from strings to shapes
+          and (ii) errors."
+  :ok stringdimmap+stringshapemap
+  :pred stringdimmap+stringshapemap-resultp
+  :prepwork ((local (in-theory (enable strip-cars)))))
