books/kestrel/remora/abstract-syntax-variable-operations.lisp
@@ -12,9 +12,10 @@
 
 (include-book "abstract-syntax-structural-operations")
 
-(include-book "kestrel/fty/string-string-map" :dir :system)
+(include-book "kestrel/fty/string-set" :dir :system)
 
 (local (include-book "kestrel/utilities/ordinals" :dir :system))
+(local (include-book "std/lists/len" :dir :system))
 
 (acl2::controlled-configuration)
 
@@ -27,115 +28,264 @@
   (xdoc::topstring
    (xdoc::p
     "These include substitutions of variables with other ASTs,
-     as well as variable renamings."))
+     as well as variable renamings.")
+   (xdoc::p
+    "The substitutions are represented as maps
+     from strings (variable names) to ASTs.
+     Since indices have distinct dimension and shape variables,
+     we use two separate maps for index variable substitutions,
+     one for dimension variables and one for shape variables.")
+   (xdoc::p
+    "The renamings are represented as maps from strings to strings.")
+   (xdoc::p
+    "Dimensions contain dimension variables,
+     but no shape or type or term variables;
+     so they only need one substitusion or renaming map
+     All the variables in a dimension are free,
+     because dimensions have no binders.")
+   (xdoc::p
+    "Shapes and indices contain dimension and shape variables,
+     but no type or term variables;
+     so they need two substitution or renaming maps.
+     All the variables in a shape or index are free,
+     because shapes and indices have no binders.")
+   (xdoc::p
+    "Types contain index (dimension and shape) and type variables,
+     but no term variables;
+     so they need three substitution or renaming maps in general,
+     but we provide separate substitution and renaming operations
+     for index and type variables in types.
+     Types have binders for both index and type variables,
+     so the operations apply to the free index and type variables;
+     when encountering bound variables,
+     they are removed from the substitution and renaming maps.")
+   (xdoc::p
+    "We also plan to add substitution and renaming operations
+     on expressions and atoms,
+     involving not only index and type variables,
+     but also term variables."))
   :order-subtopics t
   :default-parent t)
 
 ;;;;;;;;;;;;;;;;;;;;;;;;;;;;;;;;;;;;;;;;;;;;;;;;;;;;;;;;;;;;;;;;;;;;;;;;;;;;;;;;
 
-(defines subst-vars-in-indices
-  :short "Substitute variables in indices."
-  :long
-  (xdoc::topstring
-   (xdoc::p
-    "The substitution is specified by a map from strings to indices.
-     The only variables in an index are index variables.
-     All the variables in an index are free,
-     because indices have no binders."))
+(define vars-of-index-params ((params index-param-listp))
+  :returns (mv (dim-vars string-setp) (shape-vars string-setp))
+  :short "Extract the sets of dimension and shape variables
+          from a list of index parameters."
+  (b* (((when (endp params)) (mv nil nil))
+       ((mv dim-vars shape-vars) (vars-of-index-params (cdr params)))
+       (param (car params)))
+    (index-param-case
+     param
+     :dim (mv (set::insert param.name dim-vars) shape-vars)
+     :shape (mv dim-vars (set::insert param.name shape-vars))))
+  :verify-guards :after-returns)
 
-  (define subst-vars-in-index ((index indexp) (subst string-index-mapp))
-    :returns (new-index indexp)
-    :parents (abstract-syntax-variable-operations subst-vars-in-indices)
-    :short "Substitute variables in an index."
-    (index-case
-     index
-     :var (b* ((subst (string-index-map-fix subst))
-               (var+index (omap::assoc index.name subst)))
-            (if var+index
-                (cdr var+index)
-              (index-var index.name)))
-     :const (index-const index.value)
-     :shape (index-shape (subst-vars-in-index-list index.indices subst))
-     :add (index-add (subst-vars-in-index-list index.indices subst))
-     :append (index-append (subst-vars-in-index-list index.indices subst)))
-    :measure (index-count index))
+;;;;;;;;;;;;;;;;;;;;;;;;;;;;;;;;;;;;;;;;;;;;;;;;;;;;;;;;;;;;;;;;;;;;;;;;;;;;;;;;
 
-  (define subst-vars-in-index-list ((indices index-listp)
-                                    (subst string-index-mapp))
-    :returns (new-indices index-listp)
-    :parents (abstract-syntax-variable-operations subst-vars-in-indices)
-    :short "Substitute variables in a list of indices."
-    (cond ((endp indices) nil)
-          (t (cons (subst-vars-in-index (car indices) subst)
-                   (subst-vars-in-index-list (cdr indices) subst))))
-    :measure (index-list-count indices)
+(defines subst-vars-in-dims
+  :short "Substitute variables in dimensions and lists of dimensions."
+
+  ;;;;;;;;;;;;;;;;;;;;
+
+  (define subst-vars-in-dim ((dim dimp) (subst string-dim-mapp))
+    :returns (new-dim dimp)
+    :parents (abstract-syntax-variable-operations subst-vars-in-dims)
+    :short "Substitute variables in a dimension."
+    (dim-case
+     dim
+     :var (b* ((subst (string-dim-map-fix subst))
+               (var+dim (omap::assoc dim.name subst)))
+            (if var+dim
+                (cdr var+dim)
+              (dim-var dim.name)))
+     :const (dim-const dim.value)
+     :add (dim-add (subst-vars-in-dim-list dim.dims subst)))
+    :measure (dim-count dim))
+
+  ;;;;;;;;;;;;;;;;;;;;
+
+  (define subst-vars-in-dim-list ((dims dim-listp) (subst string-dim-mapp))
+    :returns (new-dims dim-listp)
+    :parents (abstract-syntax-variable-operations subst-vars-in-dims)
+    :short "Substitute variables in a list of dimensions."
+    (cond ((endp dims) nil)
+          (t (cons (subst-vars-in-dim (car dims) subst)
+                   (subst-vars-in-dim-list (cdr dims) subst))))
+    :measure (dim-list-count dims)
 
     ///
 
-    (defret len-of-subst-vars-in-index-list
-      (equal (len new-indices)
-             (len indices))
-      :hints (("Goal" :induct (len indices) :in-theory (enable len)))))
+    (defret len-of-subst-vars-in-dim-list
+      (equal (len new-dims)
+             (len dims))
+      :hints (("Goal" :induct (len dims) :in-theory (enable len)))))
+
+  ;;;;;;;;;;;;;;;;;;;;
 
   :verify-guards :after-returns
 
   ///
 
-  (fty::deffixequiv-mutual subst-vars-in-indices))
+  (fty::deffixequiv-mutual subst-vars-in-dims))
 
 ;;;;;;;;;;;;;;;;;;;;;;;;;;;;;;;;;;;;;;;;
 
-(defines subst-free-index-vars-in-types
-  :short "Substitute free index variables in types."
-  :long
-  (xdoc::topstring
-   (xdoc::p
-    "The substitution is specified by a map from strings to indices,
-     and is performed on the free variables in the indices in the types.
-     When encountering a binder of index variables,
-     the bound variables are removed from the map."))
+(defines subst-vars-in-shapes
+  :short "Substitute variables in shapes and lists of shapes."
 
-  (define subst-free-index-vars-in-type ((type typep) (subst string-index-mapp))
+  ;;;;;;;;;;;;;;;;;;;;
+
+  (define subst-vars-in-shape ((shape shapep)
+                               (subst-dim string-dim-mapp)
+                               (subst-shape string-shape-mapp))
+    :returns (new-shape shapep)
+    :parents (abstract-syntax-variable-operations subst-vars-in-shapes)
+    :short "Substitute variables in a shape."
+    (shape-case
+     shape
+     :var (b* ((subst-shape (string-shape-map-fix subst-shape))
+               (var+shape (omap::assoc shape.name subst-shape)))
+            (if var+shape
+                (cdr var+shape)
+              (shape-var shape.name)))
+     :dim (shape-dim (subst-vars-in-dim shape.dim subst-dim))
+     :dims (shape-dims (subst-vars-in-dim-list shape.dims subst-dim))
+     :append (shape-append
+              (subst-vars-in-shape-list shape.shapes subst-dim subst-shape))
+     :splice (shape-splice
+              (subst-vars-in-shape-list shape.shapes subst-dim subst-shape)))
+    :measure (shape-count shape))
+
+  ;;;;;;;;;;;;;;;;;;;;
+
+  (define subst-vars-in-shape-list ((shapes shape-listp)
+                                    (subst-dim string-dim-mapp)
+                                    (subst-shape string-shape-mapp))
+    :returns (new-shapes shape-listp)
+    :parents (abstract-syntax-variable-operations subst-vars-in-shapes)
+    :short "Substitute variables in a list of shapes."
+    (cond ((endp shapes) nil)
+          (t (cons (subst-vars-in-shape (car shapes)
+                                        subst-dim subst-shape)
+                   (subst-vars-in-shape-list (cdr shapes)
+                                             subst-dim subst-shape))))
+    :measure (shape-list-count shapes)
+
+    ///
+
+    (defret len-of-subst-vars-in-shape-list
+      (equal (len new-shapes)
+             (len shapes))
+      :hints (("Goal" :induct (len shapes) :in-theory (enable len)))))
+
+  ;;;;;;;;;;;;;;;;;;;;
+
+  :verify-guards :after-returns
+
+  ///
+
+  (fty::deffixequiv-mutual subst-vars-in-shapes))
+
+;;;;;;;;;;;;;;;;;;;;;;;;;;;;;;;;;;;;;;;;
+
+(define subst-vars-in-index ((index indexp)
+                             (subst-dim string-dim-mapp)
+                             (subst-shape string-shape-mapp))
+  :returns (new-index indexp)
+  :short "Substitute variables in an index."
+  (index-case
+   index
+   :dim (index-dim (subst-vars-in-dim index.dim subst-dim))
+   :shape (index-shape
+           (subst-vars-in-shape index.shape subst-dim subst-shape))))
+
+;;;;;;;;;;;;;;;;;;;;
+
+(define subst-vars-in-index-list ((indices index-listp)
+                                  (subst-dim string-dim-mapp)
+                                  (subst-shape string-shape-mapp))
+  :returns (new-indices index-listp)
+  :short "Substitute variables in a list of indices."
+  (cond ((endp indices) nil)
+        (t (cons
+            (subst-vars-in-index (car indices) subst-dim subst-shape)
+            (subst-vars-in-index-list (cdr indices) subst-dim subst-shape))))
+
+  ///
+
+  (defret len-of-subst-vars-in-index-list
+    (equal (len new-indices)
+           (len indices))
+    :hints (("Goal" :induct t))))
+
+;;;;;;;;;;;;;;;;;;;;;;;;;;;;;;;;;;;;;;;;;;;;;;;;;;;;;;;;;;;;;;;;;;;;;;;;;;;;;;;;
+
+(defines subst-free-index-vars-in-types
+  :short "Substitute free index variables in types and lists of types."
+
+  (define subst-free-index-vars-in-type ((type typep)
+                                         (subst-dim string-dim-mapp)
+                                         (subst-shape string-shape-mapp))
     :returns (new-type typep)
     :parents (abstract-syntax-variable-operations
               subst-free-index-vars-in-types)
     :short "Substitute free index variables in a type."
     (type-case
      type
-     :var (type-var type.name)
-     :base (type-base type.type)
-     :array (make-type-array
-             :type (subst-free-index-vars-in-type type.type subst)
-             :index (subst-vars-in-index type.index subst))
-     :fun (make-type-fun
-           :in (subst-free-index-vars-in-type-list type.in subst)
-           :out (subst-free-index-vars-in-type type.out subst))
-     :forall (make-type-forall
-              :vars type.vars
-              :type (subst-free-index-vars-in-type type.type subst))
-     :pi (b* ((bound-vars (set::mergesort (sorted-var-list->var type.vars)))
-              (subst (omap::delete* bound-vars
-                                    (string-index-map-fix subst))))
-           (make-type-pi
-            :vars type.vars
-            :type (subst-free-index-vars-in-type type.type subst)))
-     :sigma (b* ((bound-vars (set::mergesort (sorted-var-list->var type.vars)))
-                 (subst (omap::delete* bound-vars
-                                       (string-index-map-fix subst))))
-              (make-type-sigma
-               :vars type.vars
-               :type (subst-free-index-vars-in-type type.type subst))))
+     :var
+     (type-var type.name)
+     :base
+     (type-base type.type)
+     :array
+     (make-type-array
+      :type (subst-free-index-vars-in-type type.type subst-dim subst-shape)
+      :shape (subst-vars-in-shape type.shape subst-dim subst-shape))
+     :fun
+     (make-type-fun
+      :in (subst-free-index-vars-in-type-list type.in subst-dim subst-shape)
+      :out (subst-free-index-vars-in-type type.out subst-dim subst-shape))
+     :forall
+     (make-type-forall
+      :vars type.vars
+      :type (subst-free-index-vars-in-type type.type subst-dim subst-shape))
+     :pi
+     (b* (((mv bound-dim-vars bound-shape-vars)
+           (vars-of-index-params type.params))
+          (subst-dim
+           (omap::delete* bound-dim-vars (string-dim-map-fix subst-dim)))
+          (subst-shape
+           (omap::delete* bound-shape-vars (string-shape-map-fix subst-shape))))
+       (make-type-pi
+        :params type.params
+        :type (subst-free-index-vars-in-type type.type subst-dim subst-shape)))
+     :sigma
+     (b* (((mv bound-dim-vars bound-shape-vars)
+           (vars-of-index-params type.params))
+          (subst-dim
+           (omap::delete* bound-dim-vars (string-dim-map-fix subst-dim)))
+          (subst-shape
+           (omap::delete* bound-shape-vars (string-shape-map-fix subst-shape))))
+       (make-type-sigma
+        :params type.params
+        :type (subst-free-index-vars-in-type type.type subst-dim subst-shape))))
     :measure (type-count type))
 
   (define subst-free-index-vars-in-type-list ((types type-listp)
-                                              (subst string-index-mapp))
+                                              (subst-dim string-dim-mapp)
+                                              (subst-shape string-shape-mapp))
     :returns (new-types type-listp)
     :parents (abstract-syntax-variable-operations
               subst-free-index-vars-in-types)
     :short "Substitute free index variables in a list of types."
     (cond ((endp types) nil)
-          (t (cons (subst-free-index-vars-in-type (car types) subst)
-                   (subst-free-index-vars-in-type-list (cdr types) subst))))
+          (t (cons (subst-free-index-vars-in-type (car types)
+                                                  subst-dim
+                                                  subst-shape)
+                   (subst-free-index-vars-in-type-list (cdr types)
+                                                       subst-dim
+                                                       subst-shape))))
     :measure (type-list-count types)
 
     ///
@@ -155,13 +305,6 @@
 
 (defines subst-free-type-vars-in-types
   :short "Substitute free type variables in types."
-  :long
-  (xdoc::topstring
-   (xdoc::p
-    "The substitution is specified by a map from strings to types,
-     and is performed on the free variables in the types.
-     When encountering a binder of type variables,
-     the bound variables are removed from the map."))
 
   (define subst-free-type-vars-in-type ((type typep) (subst string-type-mapp))
     :returns (new-type typep)
@@ -178,7 +321,7 @@
      :base (type-base type.type)
      :array (make-type-array
              :type (subst-free-type-vars-in-type type.type subst)
-             :index type.index)
+             :shape type.shape)
      :fun (make-type-fun
            :in (subst-free-type-vars-in-type-list type.in subst)
            :out (subst-free-type-vars-in-type type.out subst))
@@ -189,10 +332,10 @@
                 :vars type.vars
                 :type (subst-free-type-vars-in-type type.type subst)))
      :pi (make-type-pi
-          :vars type.vars
+          :params type.params
           :type (subst-free-type-vars-in-type type.type subst))
      :sigma (make-type-sigma
-             :vars type.vars
+             :params type.params
              :type (subst-free-type-vars-in-type type.type subst)))
     :measure (type-count type))
 
@@ -222,110 +365,237 @@
 
 ;;;;;;;;;;;;;;;;;;;;;;;;;;;;;;;;;;;;;;;;;;;;;;;;;;;;;;;;;;;;;;;;;;;;;;;;;;;;;;;;
 
-(defines rename-vars-in-indices
-  :short "Rename variables in indices."
-  :long
-  (xdoc::topstring
-   (xdoc::p
-    "The renaming is specified by a map from strings to strings.
-     The only variables in an index are index variables.
-     All the variables in an index are free,
-     because indices have no binders."))
+(defines rename-vars-in-dims
+  :short "Rename variables in dimensions and lists of dimensions."
 
-  (define rename-vars-in-index ((index indexp) (renaming string-string-mapp))
-    :returns (new-index indexp)
-    :parents (abstract-syntax-variable-operations rename-vars-in-indices)
-    :short "Rename variables in an index."
-    (index-case
-     index
+  ;;;;;;;;;;;;;;;;;;;;
+
+  (define rename-vars-in-dim ((dim dimp) (renaming string-string-mapp))
+    :returns (new-dim dimp)
+    :parents (abstract-syntax-variable-operations rename-vars-in-dims)
+    :short "Rename variables in a dimension."
+    (dim-case
+     dim
      :var (b* ((renaming (string-string-map-fix renaming))
-               (var+name (omap::assoc index.name renaming)))
+               (var+name (omap::assoc dim.name renaming)))
             (if var+name
-                (index-var (cdr var+name))
-              (index-var index.name)))
-     :const (index-const index.value)
-     :shape (index-shape (rename-vars-in-index-list index.indices renaming))
-     :add (index-add (rename-vars-in-index-list index.indices renaming))
-     :append (index-append (rename-vars-in-index-list index.indices renaming)))
-    :measure (index-count index))
+                (dim-var (cdr var+name))
+              (dim-var dim.name)))
+     :const (dim-const dim.value)
+     :add (dim-add (rename-vars-in-dim-list dim.dims renaming)))
+    :measure (dim-count dim))
 
-  (define rename-vars-in-index-list ((indices index-listp)
-                                     (renaming string-string-mapp))
-    :returns (new-indices index-listp)
-    :parents (abstract-syntax-variable-operations rename-vars-in-indices)
-    :short "Rename variables in a list of indices."
-    (cond ((endp indices) nil)
-          (t (cons (rename-vars-in-index (car indices) renaming)
-                   (rename-vars-in-index-list (cdr indices) renaming))))
-    :measure (index-list-count indices)
+  ;;;;;;;;;;;;;;;;;;;;
+
+  (define rename-vars-in-dim-list ((dims dim-listp)
+                                   (renaming string-string-mapp))
+    :returns (new-dims dim-listp)
+    :parents (abstract-syntax-variable-operations rename-vars-in-dims)
+    :short "Rename variables in a list of dimensions."
+    (cond ((endp dims) nil)
+          (t (cons (rename-vars-in-dim (car dims) renaming)
+                   (rename-vars-in-dim-list (cdr dims) renaming))))
+    :measure (dim-list-count dims)
 
     ///
 
-    (defret len-of-rename-vars-in-index-list
-      (equal (len new-indices)
-             (len indices))
-      :hints (("Goal" :induct (len indices) :in-theory (enable len)))))
+    (defret len-of-rename-vars-in-dim-list
+      (equal (len new-dims)
+             (len dims))
+      :hints (("Goal" :induct (len dims) :in-theory (enable len)))))
+
+  ;;;;;;;;;;;;;;;;;;;;
 
   :verify-guards :after-returns
 
   ///
 
-  (fty::deffixequiv-mutual rename-vars-in-indices))
+  (fty::deffixequiv-mutual rename-vars-in-dims))
+
+;;;;;;;;;;;;;;;;;;;;;;;;;;;;;;;;;;;;;;;;
+
+(defines rename-vars-in-shapes
+  :short "Rename variables in shapes and lists of shapes."
+
+  ;;;;;;;;;;;;;;;;;;;;
+
+  (define rename-vars-in-shape ((shape shapep)
+                                (renaming-dim string-string-mapp)
+                                (renaming-shape string-string-mapp))
+    :returns (new-shape shapep)
+    :parents (abstract-syntax-variable-operations rename-vars-in-shapes)
+    :short "Rename variables in a shape."
+    (shape-case
+     shape
+     :var (b* ((renaming-shape (string-string-map-fix renaming-shape))
+               (var+name (omap::assoc shape.name renaming-shape)))
+            (if var+name
+                (shape-var (cdr var+name))
+              (shape-var shape.name)))
+     :dim (shape-dim (rename-vars-in-dim shape.dim renaming-dim))
+     :dims (shape-dims (rename-vars-in-dim-list shape.dims renaming-dim))
+     :append (shape-append (rename-vars-in-shape-list shape.shapes
+                                                      renaming-dim
+                                                      renaming-shape))
+     :splice (shape-splice (rename-vars-in-shape-list shape.shapes
+                                                      renaming-dim
+                                                      renaming-shape)))
+    :measure (shape-count shape))
+
+  ;;;;;;;;;;;;;;;;;;;;
+
+  (define rename-vars-in-shape-list ((shapes shape-listp)
+                                     (renaming-dim string-string-mapp)
+                                     (renaming-shape string-string-mapp))
+    :returns (new-shapes shape-listp)
+    :parents (abstract-syntax-variable-operations rename-vars-in-shapes)
+    :short "Rename variables in a list of shapes."
+    (cond ((endp shapes) nil)
+          (t (cons (rename-vars-in-shape (car shapes)
+                                         renaming-dim renaming-shape)
+                   (rename-vars-in-shape-list (cdr shapes)
+                                              renaming-dim renaming-shape))))
+    :measure (shape-list-count shapes)
+
+    ///
+
+    (defret len-of-rename-vars-in-shape-list
+      (equal (len new-shapes)
+             (len shapes))
+      :hints (("Goal" :induct (len shapes) :in-theory (enable len)))))
+
+  ;;;;;;;;;;;;;;;;;;;;
+
+  :verify-guards :after-returns
+
+  ///
+
+  (fty::deffixequiv-mutual rename-vars-in-shapes))
+
+;;;;;;;;;;;;;;;;;;;;;;;;;;;;;;;;;;;;;;;;
+
+(define rename-vars-in-index ((index indexp)
+                              (renaming-dim string-string-mapp)
+                              (renaming-shape string-string-mapp))
+    :returns (new-index indexp)
+    :short "Rename variables in an index."
+    (index-case
+     index
+     :dim (index-dim (rename-vars-in-dim index.dim renaming-dim))
+     :shape (index-shape
+             (rename-vars-in-shape index.shape renaming-dim renaming-shape))))
+
+;;;;;;;;;;;;;;;;;;;;
+
+(define rename-vars-in-index-list ((indices index-listp)
+                                   (renaming-dim string-string-mapp)
+                                   (renaming-shape string-string-mapp))
+  :returns (new-indices index-listp)
+  :short "Rename variables in a list of indices."
+  (cond ((endp indices) nil)
+        (t (cons (rename-vars-in-index (car indices)
+                                       renaming-dim
+                                       renaming-shape)
+                 (rename-vars-in-index-list (cdr indices)
+                                            renaming-dim
+                                            renaming-shape))))
+
+  ///
+
+  (defret len-of-rename-vars-in-index-list
+    (equal (len new-indices)
+           (len indices))
+    :hints (("Goal" :induct t))))
 
 ;;;;;;;;;;;;;;;;;;;;;;;;;;;;;;;;;;;;;;;;
 
 (defines rename-free-index-vars-in-types
   :short "Rename free index variables in types."
-  :long
-  (xdoc::topstring
-   (xdoc::p
-    "The reanming is specified by a map from strings to strings,
-     and is performed on the free variables in the indices in the types.
-     When encountering a binder of index variables,
-     the bound variables are removed from the map."))
+
+  ;;;;;;;;;;;;;;;;;;;;
 
   (define rename-free-index-vars-in-type ((type typep)
-                                          (renaming string-string-mapp))
+                                          (renaming-dim string-string-mapp)
+                                          (renaming-shape string-string-mapp))
     :returns (new-type typep)
     :parents (abstract-syntax-variable-operations
               rename-free-index-vars-in-types)
     :short "Rename free index variables in a type."
     (type-case
      type
-     :var (type-var type.name)
-     :base (type-base type.type)
-     :array (make-type-array
-             :type (rename-free-index-vars-in-type type.type renaming)
-             :index (rename-vars-in-index type.index renaming))
-     :fun (make-type-fun
-           :in (rename-free-index-vars-in-type-list type.in renaming)
-           :out (rename-free-index-vars-in-type type.out renaming))
-     :forall (make-type-forall
-              :vars type.vars
-              :type (rename-free-index-vars-in-type type.type renaming))
-     :pi (b* ((bound-vars (set::mergesort (sorted-var-list->var type.vars)))
-              (renaming (omap::delete* bound-vars
-                                    (string-string-map-fix renaming))))
-           (make-type-pi
-            :vars type.vars
-            :type (rename-free-index-vars-in-type type.type renaming)))
-     :sigma (b* ((bound-vars (set::mergesort (sorted-var-list->var type.vars)))
-                 (renaming (omap::delete* bound-vars
-                                       (string-string-map-fix renaming))))
-              (make-type-sigma
-               :vars type.vars
-               :type (rename-free-index-vars-in-type type.type renaming))))
+     :var
+     (type-var type.name)
+     :base
+     (type-base type.type)
+     :array
+     (make-type-array
+      :type (rename-free-index-vars-in-type type.type
+                                            renaming-dim
+                                            renaming-shape)
+      :shape (rename-vars-in-shape type.shape
+                                   renaming-dim
+                                   renaming-shape))
+     :fun
+     (make-type-fun
+      :in (rename-free-index-vars-in-type-list type.in
+                                               renaming-dim
+                                               renaming-shape)
+      :out (rename-free-index-vars-in-type type.out
+                                           renaming-dim
+                                           renaming-shape))
+     :forall
+     (make-type-forall
+      :vars type.vars
+      :type (rename-free-index-vars-in-type type.type
+                                            renaming-dim
+                                            renaming-shape))
+     :pi
+     (b* (((mv bound-dim-vars bound-shape-vars)
+           (vars-of-index-params type.params))
+          (renaming-dim
+           (omap::delete* bound-dim-vars
+                          (string-string-map-fix renaming-dim)))
+          (renaming-shape
+           (omap::delete* bound-shape-vars
+                          (string-string-map-fix renaming-shape))))
+       (make-type-pi
+        :params type.params
+        :type (rename-free-index-vars-in-type type.type
+                                              renaming-dim
+                                              renaming-shape)))
+     :sigma
+     (b* (((mv bound-dim-vars bound-shape-vars)
+           (vars-of-index-params type.params))
+          (renaming-dim
+           (omap::delete* bound-dim-vars
+                          (string-string-map-fix renaming-dim)))
+          (renaming-shape
+           (omap::delete* bound-shape-vars
+                          (string-string-map-fix renaming-shape))))
+       (make-type-sigma
+        :params type.params
+        :type (rename-free-index-vars-in-type type.type
+                                              renaming-dim
+                                              renaming-shape))))
     :measure (type-count type))
 
-  (define rename-free-index-vars-in-type-list ((types type-listp)
-                                               (renaming string-string-mapp))
+  ;;;;;;;;;;;;;;;;;;;;
+
+  (define rename-free-index-vars-in-type-list
+    ((types type-listp)
+     (renaming-dim string-string-mapp)
+     (renaming-shape string-string-mapp))
     :returns (new-types type-listp)
     :parents (abstract-syntax-variable-operations
               rename-free-index-vars-in-types)
     :short "Rename free index variables in a list of types."
     (cond ((endp types) nil)
-          (t (cons (rename-free-index-vars-in-type (car types) renaming)
-                   (rename-free-index-vars-in-type-list (cdr types) renaming))))
+          (t (cons (rename-free-index-vars-in-type (car types)
+                                                   renaming-dim
+                                                   renaming-shape)
+                   (rename-free-index-vars-in-type-list (cdr types)
+                                                        renaming-dim
+                                                        renaming-shape))))
     :measure (type-list-count types)
 
     ///
@@ -334,6 +604,8 @@
       (equal (len new-types)
              (len types))
       :hints (("Goal" :induct (len types) :in-theory (enable len)))))
+
+  ;;;;;;;;;;;;;;;;;;;;
 
   :verify-guards :after-returns
 
@@ -345,20 +617,13 @@
 
 (defines rename-free-type-vars-in-types
   :short "Rename free type variables in types."
-  :long
-  (xdoc::topstring
-   (xdoc::p
-    "The renaming is specified by a map from strings to strings,
-     and is performed on the free variables in the types.
-     When encountering a binder of type variables,
-     the bound variables are removed from the map."))
 
   (define rename-free-type-vars-in-type ((type typep)
                                          (renaming string-string-mapp))
     :returns (new-type typep)
     :parents (abstract-syntax-variable-operations
               rename-free-type-vars-in-types)
-    :short "Reanem free index variables in a type."
+    :short "Rename free type variables in a type."
     (type-case
      type
      :var (b* ((renaming (string-string-map-fix renaming))
@@ -369,7 +634,7 @@
      :base (type-base type.type)
      :array (make-type-array
              :type (rename-free-type-vars-in-type type.type renaming)
-             :index type.index)
+             :shape type.shape)
      :fun (make-type-fun
            :in (rename-free-type-vars-in-type-list type.in renaming)
            :out (rename-free-type-vars-in-type type.out renaming))
@@ -380,10 +645,10 @@
                 :vars type.vars
                 :type (rename-free-type-vars-in-type type.type renaming)))
      :pi (make-type-pi
-          :vars type.vars
+          :params type.params
           :type (rename-free-type-vars-in-type type.type renaming))
      :sigma (make-type-sigma
-             :vars type.vars
+             :params type.params
              :type (rename-free-type-vars-in-type type.type renaming)))
     :measure (type-count type))
 
@@ -392,7 +657,7 @@
     :returns (new-types type-listp)
     :parents (abstract-syntax-variable-operations
               rename-free-type-vars-in-types)
-    :short "Rename free index variables in a list of types."
+    :short "Rename free type variables in a list of types."
     (cond ((endp types) nil)
           (t (cons (rename-free-type-vars-in-type (car types) renaming)
                    (rename-free-type-vars-in-type-list (cdr types) renaming))))
